common/Separation.v
@@ -849,7 +849,8 @@ Qed.
 
 Lemma external_call_parallel_rule:
   forall (F V: Type) ef (ge: Genv.t F V) vargs1 m1 t vres1 m1' m2 j P vargs2,
-  external_call ef ge vargs1 m1 t vres1 m1' ->
+    external_call ef ge vargs1 m1 t vres1 m1' ->
+    injection_full j m1 ->
   m2 |= minjection j m1 ** globalenv_inject ge j ** P ->
   Val.inject_list j vargs1 vargs2 ->
   exists j' vres2 m2' t',
@@ -858,14 +859,15 @@ Lemma external_call_parallel_rule:
   /\ m2' |= minjection j' m1' ** globalenv_inject ge j' ** P
   /\ inject_incr j j'
   /\ inject_separated j j' m1 m2
-  /\ inject_trace j t t'.
+  /\ inject_trace j' t t' /\
+    injection_full j m1 .
 Proof.
-  intros until vargs2; intros CALL SEP ARGS.
+  intros until vargs2; intros CALL INJFULL SEP ARGS.
   destruct SEP as (A & B & C). simpl in A. 
   exploit external_call_mem_inject; eauto.
   eapply globalenv_inject_preserves_globals. eapply sep_pick1; eauto.
   intros (j' & vres2 & m2' & t' & CALL' & RES & INJ' &
-          UNCH1 & UNCH2 & INCR & ISEP & INJT).
+          UNCH1 & UNCH2 & INCR & ISEP & INJT & INJFULL').
   assert (MAXPERMS: forall b ofs p,
             Mem.valid_block m1 b -> Mem.perm m1' b ofs Max p -> Mem.perm m1 b ofs Max p).
   { intros. eapply external_call_max_perm; eauto. }
